Prove pegexec correct for pegs that record "rightmost" error

examples/formal-languages/context-free/locationScript.sml
@@ -2,26 +2,31 @@ open HolKernel Parse boolLib bossLib
 
 val _ = new_theory "location";
 
-Datatype: locn = <| row : num;  col : num; offset : num |>
+Datatype: locn = UNKNOWNpt | EOFpt | POSN num num
 End
+
+Definition locnrow_def:
+  locnrow (POSN r c) = r
+End
+val _ = add_record_field ("row", “locnrow”)
+
+Definition locncol_def:
+  locncol (POSN r c) = c
+End
+val _ = add_record_field ("col", “locncol”)
 
 Datatype: locs = Locs locn locn
 End
 
 Definition default_loc_def:
-  default_loc = <| row := 1; col := 1; offset := 0 |>
+  default_loc = POSN 0 0
 End
 
 Definition start_locs_def: start_locs = Locs default_loc default_loc
 End
 
-Definition end_locn_def:
-  end_locn = <| row := 0; col := 0; offset := 1 |>
-End
-
-Definition unknown_locn_def:
-  unknown_locn = <| row := 0; col := 0; offset := 0 |>
-End
+Overload end_locn[local] = “EOFpt”
+Overload unknown_locn[local] = “UNKNOWNpt”
 
 Definition unknown_loc_def:
   unknown_loc = Locs unknown_locn unknown_locn
@@ -30,30 +35,41 @@ End
 Definition locnle_def:
   locnle l1 l2 <=>
     l1 = l2 ∨ (* reflexivity, for free *)
-    l1 = default_loc ∨ (* minimal element *)
+    l1 = unknown_locn ∨ (* minimal element *)
     l2 = end_locn ∨ (* maximal element *)
     (* otherwise compare row and col lexicographically*)
-    l1.row ≠ 0 ∧ l2.row ≠ 0 ∧ l1.col ≠ 0 ∧ l2.col ≠ 0 ∧
+    l2 ≠ unknown_locn ∧ l1 ≠ end_locn ∧
     (l1.row < l2.row ∨ l1.row = l2.row ∧ l1.col < l2.col)
 End
 
-Theorem locn_rwts[simp]:
-  default_loc ≠ end_locn ∧ default_loc ≠ unknown_locn ∧
-  end_locn ≠ unknown_locn ∧ end_locn.row = 0 ∧
-  unknown_locn.row = 0 ∧ default_loc.row = 1 ∧ default_loc.col = 1
+Theorem locnle_REFL[simp]:
+  locnle l l
 Proof
-  simp[default_loc_def, end_locn_def, unknown_locn_def]
+  simp[locnle_def]
 QED
 
-Theorem locnle_REFL[simp]:
-  locnle loc loc
-Proof simp[locnle_def]
+Theorem locnle_total:
+  locnle l1 l2 ∨ locnle l2 l1
+Proof
+  simp[locnle_def] >> Cases_on ‘l1 = l2’ >> simp[] >>
+  map_every Cases_on [‘l1 = unknown_locn’, ‘l2 = unknown_locn’,
+                      ‘l1 = end_locn’, ‘l2 = end_locn’] >> simp[] >>
+  reverse (Cases_on ‘l1.row = l2.row’) >> simp[] >>
+  ‘l1.col ≠ l2.col’ suffices_by simp[] >>
+  map_every Cases_on [‘l1’, ‘l2’] >> gvs[locnrow_def, locncol_def]
+QED
+
+Theorem locnle_ANTISYM:
+  locnle l1 l2 ∧ locnle l2 l1 ⇒ l1 = l2
+Proof
+  map_every Cases_on [‘l1’, ‘l2’] >> gvs[locnle_def,locnrow_def, locncol_def]
 QED
 
 Theorem locnle_TRANS:
   locnle l1 l2 ∧ locnle l2 l3 ⇒ locnle l1 l3
 Proof
-  rw[locnle_def] >> fs[]
+  map_every Cases_on [‘l1’, ‘l2’, ‘l3’] >>
+  gvs[locnle_def,locnrow_def, locncol_def]
 QED
 
 Theorem locnle_end[simp]:
@@ -62,8 +78,8 @@ Proof
   simp[locnle_def]
 QED
 
-Theorem locnle_start[simp]:
-  locnle l default_loc ⇔ l = default_loc
+Theorem locnle_unknown[simp]:
+  locnle l unknown_locn ⇔ l = unknown_locn
 Proof
   simp[locnle_def]
 QED
@@ -78,44 +94,58 @@ Proof
   Cases_on ‘l’ >> simp[]
 QED
 
-val merge_locs_def = Define`
-  merge_locs (Locs l1 l2) (Locs l3 l4) = Locs l1 l4
-`;
+Theorem locsle_total:
+  locsle l1 l2 ∨ locsle l2 l1
+Proof
+  map_every Cases_on [‘l1’, ‘l2’] >> simp[locnle_total]
+QED
 
-val merge_list_locs_def = Define`
+Theorem locsle_TRANS:
+  locsle l1 l2 ∧ locsle l2 l3 ⇒ locsle l1 l3
+Proof
+  map_every Cases_on [‘l1’, ‘l2’, ‘l3’] >> simp[] >> metis_tac[locnle_TRANS]
+QED
+
+Definition merge_locs_def:
+  merge_locs (Locs l1 l2) (Locs l3 l4) = Locs l1 l4
+End
+
+Definition merge_list_locs_def:
   (merge_list_locs [] = unknown_loc) /\
   (merge_list_locs (h :: []) = h) /\
   (merge_list_locs (h1 :: h2 :: []) = merge_locs h1 h2) /\
-  (merge_list_locs (h1 :: h2 :: t) = merge_list_locs (h1 :: t))`;
+  (merge_list_locs (h1 :: h2 :: t) = merge_list_locs (h1 :: t))
+End
 
 (* for debugging *)
 
-val map_loc_def = Define`
+Definition map_loc_def[simp]:
   (map_loc [] _ = []) /\
   (map_loc (h :: t) n =
-    (h, Locs <| row := n; col := 0; offset := 0 |>
-             <| row := n; col := 1; offset := 0 |>) :: map_loc t (n+1))
-`;
+    (h, Locs (POSN 0 n) (POSN 0 n)) :: map_loc t (n+1))
+End
 
 
-val merge_locs_assoc = Q.store_thm(
-  "merge_locs_assoc[simp]",
-  ‘(merge_locs (merge_locs l1 l2) l3 = merge_locs l1 l3) ∧
-   (merge_locs l1 (merge_locs l2 l3) = merge_locs l1 l3)’,
-  map_every Cases_on [`l1`, `l2`, `l3`] >>
-  simp[merge_locs_def]);
+Theorem merge_locs_assoc[simp]:
+  (merge_locs (merge_locs l1 l2) l3 = merge_locs l1 l3) ∧
+  (merge_locs l1 (merge_locs l2 l3) = merge_locs l1 l3)
+Proof
+  map_every Cases_on [`l1`, `l2`, `l3`] >> simp[merge_locs_def]
+QED
 
-val merge_list_locs_2 = Q.store_thm(
-  "merge_list_locs_2[simp]",
-  ‘∀h1 h2 t.
-     merge_list_locs (h1 :: h2 :: t) = merge_list_locs (merge_locs h1 h2 :: t)’,
-  Induct_on ‘t’ >> simp[merge_list_locs_def]);
+Theorem merge_list_locs_2[simp]:
+  ∀h1 h2 t.
+    merge_list_locs (h1 :: h2 :: t) = merge_list_locs (merge_locs h1 h2 :: t)
+Proof
+  Induct_on ‘t’ >> simp[merge_list_locs_def]
+QED
 
-val merge_list_locs_nested = Q.store_thm(
-  "merge_list_locs_nested[simp]",
-  ‘∀h t1 t2. merge_list_locs (merge_list_locs (h::t1) :: t2) =
-             merge_list_locs (h :: t1 ++ t2)’,
-  Induct_on ‘t1’ >> simp[merge_list_locs_def]);
+Theorem merge_list_locs_nested[simp]:
+  ∀h t1 t2. merge_list_locs (merge_list_locs (h::t1) :: t2) =
+            merge_list_locs (h :: t1 ++ t2)
+Proof
+  Induct_on ‘t1’ >> simp[merge_list_locs_def]
+QED
 
 val merge_list_locs_sing = Q.store_thm(
   "merge_list_locs_sing[simp]",
