examples/formal-languages/context-free/pegexecScript.sml
@@ -16,7 +16,8 @@ Datatype:
   | dropErr kont
   | addErr locs 'err kont
   | cmpErrs kont
-  | returnTo (('atok # locs) list) ('cvalue option list) kont
+  | cmpEO ((locs # 'err) option) kont
+  | returnTo (('atok#locs) list) ('cvalue option list) kont
   | restoreEO ((locs # 'err) option) kont
   | poplist ('cvalue list -> 'cvalue) kont
   | listsym (('atok,'bnt,'cvalue,'err) pegsym)
@@ -40,22 +41,23 @@ val poplistval_def = Define`
 
 Datatype:
   evalcase = EV (('atok,'bnt,'cvalue,'err) pegsym)
-                (('atok # locs) list)
+                (('atok#locs) list)
                 ('cvalue option list)
                 ((locs # 'err) option)
                 ((locs # 'err) list)
                 (('atok,'bnt,'cvalue,'err) kont)
                 (('atok,'bnt,'cvalue,'err) kont)
            | AP (('atok,'bnt,'cvalue,'err) kont)
-                (('atok # locs) list)
+                (('atok#locs) list)
                 ('cvalue option list)
                 ((locs # 'err) option)
                 ((locs # 'err) list)
-           | Result ((('atok # locs) list, 'cvalue, 'err) pegresult)
+           | Result ((('atok # locs)list, 'cvalue, 'err) pegresult)
            | Looped
 End
 
 Overload OME[local] = “optmax MAXerr”
+Overload EOF[local] = “Locs EOFpt EOFpt”
 
 Definition coreloop_def[nocompute]:
   coreloop G =
@@ -65,19 +67,19 @@ Definition coreloop_def[nocompute]:
                    EV (empty v) i r eo errs k fk => AP k i (SOME v::r) eo errs
                  | EV (any tf) i r eo errs k fk =>
                    (case i of
-                        [] => let err = (sloc i, G.anyEOF)
+                        [] => let err = (EOF, G.anyEOF)
                               in
-                                AP fk i r (OME (SOME err) eo) (err::errs)
-                      | h::t => AP k t (SOME (tf h) :: r) eo errs)
+                                AP fk i r (OME eo (SOME err)) (err::errs)
+                      | h::t => AP k t (SOME (tf (FST h)) :: r) eo errs)
                  | EV (tok P tf2) i r eo errs k fk =>
                    (case i of
-                        [] => let err = (sloc i, G.tokEOF)
+                        [] => let err = (EOF, G.tokEOF)
                               in
-                                AP fk i r (OME (SOME err) eo) (err::errs)
+                                AP fk i r (OME eo (SOME err)) (err::errs)
                       | h::t => if P (FST h) then
-                                  AP k t (SOME (tf2 h)::r) eo errs
+                                  AP k t (SOME (tf2 (FST h))::r) eo errs
                                 else let err = (sloc i, G.tokFALSE)
-                                     in AP fk i r (OME (SOME err) eo)
+                                     in AP fk i r (OME eo (SOME err))
                                            (err::errs))
                  | EV (nt n tf3) i r eo errs k fk =>
                    if n ∈ FDOM G.rules then
@@ -86,7 +88,10 @@ Definition coreloop_def[nocompute]:
                      Looped
                  | EV (seq e1 e2 f) i r eo errs k fk =>
                      EV e1 i r eo errs
-                        (ksym e2 (appf2 f k) (returnTo i r fk))
+                        (restoreEO eo
+                         (ksym e2
+                          (appf2 f k)
+                          (cmpEO eo $ returnTo i r fk)))
                         fk
                  | EV (choice e1 e2 cf) i r eo errs k fk =>
                      EV e1 i r eo errs
@@ -96,7 +101,9 @@ Definition coreloop_def[nocompute]:
                           (dropErr (appf1 (cf o INR) k))
                           (cmpErrs fk)))
                  | EV (rpt e lf) i r eo errs k fk =>
-                     EV e i (NONE::r) eo errs (listsym e lf k) (poplist lf k)
+                     EV e i (NONE::r) eo errs
+                        (restoreEO eo $ listsym e lf k)
+                        (poplist lf k)
                  | EV (not e v) i r eo errs k fk =>
                      EV e i r eo errs
                         (restoreEO eo $
@@ -105,7 +112,7 @@ Definition coreloop_def[nocompute]:
                  | EV (error err) i r eo errs k fk =>
                      let err = (sloc i, err)
                      in
-                       AP fk i r (OME (SOME err) eo) (err :: errs)
+                       AP fk i r (OME eo (SOME err)) (err :: errs)
                  | AP done i [] _ _ => Looped
                  | AP done i (NONE :: t) _ _ => Looped
                  | AP done i (SOME rv :: _) eo _ => Result (Success i rv eo)
@@ -114,13 +121,15 @@ Definition coreloop_def[nocompute]:
                  | AP (dropErr _) i r _ [] => Looped
                  | AP (dropErr k) i r eo (_ :: t) => AP k i r eo t
                  | AP (addErr l e k) i r eo errs =>
-                     AP k i r (OME (SOME (l,e)) eo) ((l,e)::errs)
+                     AP k i r (OME eo (SOME (l,e))) ((l,e)::errs)
                  | AP (cmpErrs k) i r _ [] => Looped
                  | AP (cmpErrs k) i r _ [_] => Looped
                  | AP (cmpErrs k) i r eo ((l2,er2)::(l1,er1)::rest) =>
                      AP k i r eo
-                        ((if locsle l1 l2 then (l2,er2) else (l1,er1)) ::
-                         rest)
+                        ((if locsle l1 l2 then (l2,er2) else (l1,er1)) :: rest)
+                 | AP (cmpEO eo1 k) i r eo2 [] => Looped
+                 | AP (cmpEO eo1 k) i r eo2 ((l,err)::rest) =>
+                     AP k i r (OME eo1 (SOME (l,err))) ((l,err)::rest)
                  | AP (ksym e k fk) i r eo errs => EV e i r eo errs k fk
                  | AP (appf1 f1 k) i (SOME v :: r) eo errs =>
                      AP k i (SOME (f1 v) :: r) eo errs
@@ -131,10 +140,10 @@ Definition coreloop_def[nocompute]:
                  | AP (returnTo i r k) i' r' eo errs => AP k i r eo errs
                  | AP (restoreEO eo k) i r eo' errs => AP k i r eo errs
                  | AP (listsym e f k) i r eo errs =>
-                     EV e i r eo errs (listsym e f k) (poplist f k)
+                     EV e i r eo errs (restoreEO eo $ listsym e f k) (poplist f k)
                  | AP (poplist f k) i r eo [] => Looped
                  | AP (poplist f k) i r eo (e :: errs) =>
-                     AP k i (poplistval f r) (OME (SOME e) eo) errs
+                     AP k i (poplistval f r) eo errs
                  | Result r => Result r
                  | Looped => Looped)
 End
@@ -237,7 +246,8 @@ val better_apply =
          ([`k` |-> `poplist f k`, ‘errs’ |-> ‘[]’], []),
          ([`k` |-> `poplist f k`, ‘errs’ |-> ‘le::errs’], []),
          ([`k` |-> `listsym e f k`], []),
-         ([‘k’ |-> ‘restoreEO eo0 k’], [])
+         ([‘k’ |-> ‘restoreEO eo0 k’], []),
+         ([‘k’ |-> ‘cmpEO eo0 k’, ‘errs’ |-> ‘(l,err)::errs’], [])
          ]
 
 Theorem peg_nt_thm =
@@ -257,6 +267,21 @@ Proof
   Cases_on ‘eo’ >> simp[optmax_def]
 QED
 
+Theorem OME_ASSOC[local,simp]:
+  OME eo1 (OME eo2 eo3) = OME (OME eo1 eo2) eo3
+Proof
+  map_every Cases_on [‘eo1’, ‘eo2’, ‘eo3’] >> simp[optmax_def] >>
+  rename [‘MAXerr e1 (MAXerr e2 e3)’] >>
+  map_every Cases_on [‘e1’, ‘e2’, ‘e3’] >> rw[MAXerr_def] >>
+  metis_tac[locsle_total,locsle_TRANS]
+QED
+
+Theorem MAXerr_id[simp]:
+  MAXerr x x = x
+Proof
+  Cases_on ‘x’ >> simp[MAXerr_def]
+QED
+
 Theorem exec_correct0[local]:
   (∀i e r.
      peg_eval G (i,e) r ⇒
@@ -274,22 +299,23 @@ Theorem exec_correct0[local]:
        peg_exec G e i (MAP SOME vs ++ (NONE::stk))
                 eo
                 errs
-                (listsym e f k)
+                (restoreEO eo $ listsym e f k)
                 (poplist f k) =
        applykont G k j (SOME (f (REVERSE vs ++ vlist)) :: stk)
                  (OME eo (SOME err))
                  errs)
 Proof
-  ho_match_mp_tac peg_eval_strongind' >>
-  simp[peg_exec_thm, peg_nt_thm, applykont_thm, FORALL_result, AllCaseEqs()] >>
-
-  simp[peg_exec_thm, FORALL_result, applykont_thm]
-  rpt conj_tac
-  >- ((* locsle comparison *) rw[])
+  ho_match_mp_tac peg_eval_strongind' >> rpt conj_tac >>
+  simp[peg_exec_thm, peg_nt_thm, applykont_thm, FORALL_result, AllCaseEqs(),
+       arithmeticTheory.ADD1, MAXerr_def, pairTheory.FORALL_PROD]
+  >- ((* locsle comparison *) rw[optmax_def, MAXerr_def] >>
+      simp[Excl "OME_ASSOC", GSYM OME_ASSOC, optmax_def, MAXerr_def])
   >- ((* rpt - no elements succeed *)
-      map_every qx_gen_tac [`e`, `f`, `i`, `j`, `vlist`] >> strip_tac >>
-      map_every qx_gen_tac [`k`, `stk`, ‘errs’] >>
-      first_x_assum (qspecl_then [`f`, `k`, `stk`, ‘errs’, `[]`] mp_tac) >>
+      map_every qx_gen_tac [`e`, `f`, `i`, `j`, `vlist`, ‘errl’, ‘err’] >>
+      strip_tac >>
+      map_every qx_gen_tac [‘eo0’, `k`, `stk`, ‘errs’] >>
+      first_x_assum (qspecl_then [`f`, `k`, `stk`, ‘eo0’, ‘errs’, `[]`]
+                     mp_tac) >>
       simp[])
   >- ((* poplistval works *)
       rpt strip_tac >> rpt (AP_TERM_TAC ORELSE AP_THM_TAC) >>
@@ -303,9 +329,11 @@ Proof
                      (REVERSE vs ++ a, stk)` >- simp[] >>
       Induct_on `vs` >> simp[poplist_aux_def])
   >- ((* rpt - some elements succeed *)
-      map_every qx_gen_tac [`e`, `i0`, `i1`, `j`, `v`, `vs`] >> strip_tac >>
-      map_every qx_gen_tac [`f`, `k`, `stk`, ‘errs’, `vs'`] >>
-      first_x_assum (qspecl_then [`f`, `k`, `stk`, ‘errs’, `v::vs'`] mp_tac) >>
+      map_every qx_gen_tac [`e`, ‘eo0’, ‘errl’, ‘err’, `i0`, `i1`, `j`, `v`, `vs`] >>
+      strip_tac >>
+      map_every qx_gen_tac [`f`, `k`, `stk`, ‘eo’, ‘errs’, `vs'`] >>
+      first_x_assum (qspecl_then [`f`, `k`, `stk`, ‘eo’, ‘errs’,
+                                  `v::vs'`] mp_tac) >>
       simp[] >>
       simp_tac bool_ss [GSYM listTheory.APPEND_ASSOC, listTheory.APPEND])
 QED
@@ -331,7 +359,7 @@ val option_CASES = optionTheory.option_nchotomy
 val list_CASES = listTheory.list_CASES
 
 Theorem pegexec:
-  peg_eval G (s,e) r ⇒ peg_exec G e s [] [] done failed = Result r
+  peg_eval G (s,e) r ⇒ peg_exec G e s [] NONE [] done failed = Result r
 Proof
   strip_tac >>
   Cases_on ‘r’ >> (drule pegexec_succeeds ORELSE drule pegexec_fails) >>
@@ -340,7 +368,7 @@ QED
 
 Theorem peg_eval_executed:
   wfG G ∧ e ∈ Gexprs G ⇒
-    (peg_eval G (s,e) r ⇔ peg_exec G e s [] [] done failed = Result r)
+    (peg_eval G (s,e) r ⇔ peg_exec G e s [] NONE [] done failed = Result r)
 Proof
   strip_tac >> eq_tac >- simp[pegexec] >>
   strip_tac >>
@@ -355,15 +383,15 @@ End
 Definition pegparse_def:
   pegparse G s =
     if wfG G then
-      case destResult (peg_exec G G.start s [] [] done failed) of
-        Success s v => SOME (s,v)
+      case destResult (peg_exec G G.start s [] NONE [] done failed) of
+        Success s v eo => SOME (s,v,eo)
       | _ => NONE
     else NONE
 End
 
 Theorem pegparse_eq_SOME:
-  pegparse G s = SOME (s', v) ⇔
-  wfG G ∧ peg_eval G (s,G.start) (Success s' v)
+  pegparse G s = SOME (s', v, eo) ⇔
+  wfG G ∧ peg_eval G (s,G.start) (Success s' v eo)
 Proof
   Tactical.REVERSE (Cases_on `wfG G`) >- simp[pegparse_def] >>
   `∃r. peg_eval G (s,G.start) r`
@@ -388,7 +416,7 @@ Proof
 QED
 
 Theorem peg_exec_total:
-  wfG G ==> ∃r. peg_exec G G.start i [] [] done failed = Result r
+  wfG G ==> ∃r. peg_exec G G.start i [] NONE [] done failed = Result r
 Proof
   strip_tac >>
   `∃pr. peg_eval G (i, G.start) pr` by simp[peg_eval_total, start_IN_Gexprs] >>
@@ -398,7 +426,7 @@ QED
 (*
    |- wfG G ⇒
       ∃r.
-        coreloop G (pegexec$EV G.start i [] done failed) = SOME (Result r)
+        coreloop G (pegexec$EV G.start i [] NONE [] done failed) = SOME (Result r)
 *)
 Theorem coreloop_total =
   peg_exec_total |> SIMP_RULE (srw_ss()) [peg_exec_def, AllCaseEqs()]
